  \solution{
Extension of Tseitin's Transformation:\\
\begin{enumerate}
\item
Clauses for the equivalence-connective $\IFF$: \\
First we replace $\IFF$ by $\IMPL$ using the rule\\
\begin{equation*}
(a \IFF b)=(a \IMPL b)\AND(b \IMPL a)
\end{equation*}

Thus, the equivalence can be written as follows:\\
\begin{eqnarray*}
l_i \IFF (l_{i'} \IFF l_{i''})\\
= (l_i \IMPL (l_{i'} \IFF l_{i''})) \AND ((l_{i'} \IFF l_{i''}) \IMPL l_{i})\\
= [l_i \IMPL ((l_{i'} \IFF l_{i''}) \AND (l_{i''} \IMPL l_{i'}))] 
\AND [((l_{i'} \IMPL l_{i''}) \AND (l_{i''} \IMPL l_{i'})) \IMPL l_i]\\
= [(l_i \IMPL (l_{i'} \IMPL l_{i''})) \AND (l_i \IMPL (l_{i''} \IMPL l_{i'}))] 
\AND [((l_{i'} \IMPL l_{i''}) \IMPL l_i) \AND ((l_{i''} \IMPL l_{i'}) \IMPL l_i)]\\
= [(l_i \IMPL (\neg l_{i'} \OR l_{i''})) \AND (l_i \IMPL (\neg l_{i''} \OR l_{i'}))] 
\AND [((l_{i'} \AND\neg l_{i''}) \OR l_i) \AND ((l_{i''} \AND\neg l_{i'}) \OR l_i)]\\
= [(\neg l_i \OR (\neg l_{i'} \OR l_{i''})) \AND (\neg l_i \OR (\neg l_{i''} \OR l_{i'}))] 
\AND [((l_{i'} \AND\neg l_{i''}) \AND (l_{i''} \AND\neg l_{i'})) \OR l_{i}]\\
= [(\neg l_i \OR \neg l_{i'} \OR l_{i''}) \AND (\neg l_i \OR \neg l_{i''} \OR l_{i'})] 
\AND [((l_{i'} \AND l_{i''}) \AND (\neg l_{i'} \AND\neg l_{i''})) \OR l_{i}]\\
= (\neg l_i \OR \neg l_{i'} \OR l_{i''}) \AND (\neg l_i \OR \neg l_{i''} \OR l_{i'}) 
\AND [((\neg l_{i'} \OR \neg l_{i''}) \AND (l_{i'} \OR l_{i''})) \OR l_{i}]\\
= (\neg l_i \OR \neg l_{i'} \OR l_{i''}) \AND (\neg l_i \OR \neg l_{i''} \OR l_{i'}) 
\AND (l_{i} \OR \neg l_{i'} \OR \neg l_{i''}) \AND (l_{i} \OR l_{i'} \OR l_{i''})\\
\end{eqnarray*}

Now we can construct the table with the equivalences for the SFOs and the 
associated clauses in CNF (local constraints):

% use packages: array
\begin{tabular}{|l|l|l|l|1|}
\hline
\textsl{\small Equivalences} & \multicolumn{4}{c|}{\textsl{\small Associated
Clauses}} \\ 
{\small \textsl{for SFOs in} $\IFF $} & $C_{1}(\IFF )$ & $C_{2}(\IFF )$ & $%
C_{3}(\IFF )$ & $C_{4}(\IFF )$ \\ \hline
$l_{i}\IFF(l_{i'}\IFF l_{i''})$ & $\lnot l_{i}\OR \neg l_{i'}\OR l_{i''}$ & 
$\lnot l_{i}\OR l_{i'}\OR \neg l_{i''}$ & $l_{i}\OR\neg l_{i'}\OR\neg l_{i''}$ & 
$l_i\OR l_{i'}\OR l_{i''}$ \\ \hline
\end{tabular}
\label{tab:translation_cnf}

\bigskip
\item
Clauses for the XOR-connective $\oplus$: \\
We replace $\oplus$ by $\IMPL$ using the substitution rule:
\begin{eqnarray*}
l_{k'} \oplus l_{k''}\\
= \neg(l_{k'} \IMPL l_{k''}) \OR \neg (l_{k''} \IMPL l_{k'})\\
\text{(which is the dual problem of i):)}\\
= \neg((l_{k'} \IMPL l_{k''}) \AND (l_{k''} \IMPL l_{k'}))\\ 
\end{eqnarray*}

\end{enumerate}

  }