
\textbf{Solution:}\\
Since the TPL language describes a context free grammar, 
we can construct any program due to parsing of the production rules (nonterminals). Hence

\begin{small}
\begin{eqnarray*}
\mathcal{P} &\Rightarrow &\mathcal{P};\mathcal{P} \\
&\Rightarrow &\mathcal{V}:=\mathcal{E};\mathcal{P} \\
& \Rightarrow &x:=(\mathcal{E}\ \mathcal{B}\ \mathcal{E});\mathcal{P} \\
&\Rightarrow &x:=(\mathcal{V}+\mathcal{V});\mathcal{P} \\
&\Rightarrow &x:=x+y;\ \mathcal{P} \\
&\Rightarrow &x:=x + y; \IF\ \mathcal{E}\ \THEN\ \mathcal{P}\ \ELSE\ \mathcal{P}\ \FI\ \\
&\Rightarrow & x:=x + y; \IF\ (\mathcal{E}\ \mathcal{B}\ \mathcal{E})\ \THEN\ 
 \mathcal{P}\ \ELSE\ \mathcal{Q}\ \IF\ \\
&\Rightarrow & x:=x + y; \IF\ (\mathcal{V}<\mathcal{N})\ \THEN\ \mathcal{P}
  \ELSE\ \mathcal{Q}\ \FI\ \\
% 
&\Rightarrow & x:=x + y; \IF\ (x < 0)\ \THEN\ \mathcal{P}\ \ELSE\ \mathcal{Q%
 }\ \FI\ \\
% 
&\Rightarrow & x:=x + y; \IF\ (x < 0)\ \THEN\ \ABORT; \ELSE\ \mathcal{Q}\ \FI\ \\
% 
&\Rightarrow & x:=x + y; \IF\ (x < 0)\ \THEN\ \ABORT; \ELSE\ \WHILE\ \mathcal{E}
 \ \DO\ \mathcal{P}\ \OD\ \FI\ \\
% 
&\Rightarrow & x:=x + y; \IF\ (x < 0)\ \THEN\ \ABORT; \ELSE\ \WHILE\ (\mathcal{E%
 }\ \mathcal{B}\ \mathcal{E})\ \DO\ \mathcal{P}\ \OD\ \FI\ \\
% 
% &\Rightarrow & x:=x + y; \IF\ (x < 0)\ \THEN\ \ABORT; \ELSE\ \WHILE\ (\mathcal{E%
%  }\neq \mathcal{E})\ \DO\ \mathcal{P}\ \OD\ \FI\ \\
% % 
% &\Rightarrow & x:=x + y; \IF\ (x < 0)\ \THEN\ \ABORT; \ELSE\ \WHILE\ (\mathcal{V%
%  }\neq \mathcal{E})\ \DO\ \mathcal{P}\ \OD\ \FI\ \\
% % 
% &\Rightarrow & x:=x + y; \IF\ (x < 0)\ \THEN\ \ABORT; \ELSE\ \WHILE\ (\mathcal{V%
%  }\neq \mathcal{V})\ \DO\ \mathcal{P}\ \OD\ \FI\ \\
% 
&\Rightarrow & x:=x + y; \IF\ (x < 0)\ \THEN\ \ABORT; \ELSE\ \WHILE\ (x\neq y)
\ \DO\ \mathcal{P};\mathcal{P}\ \OD\ \FI\ \\
% 
&\Rightarrow & x:=x + y; \IF\ (x < 0)\ \THEN\ \ABORT; \ELSE\ \WHILE\ (x\neq y)
\ \DO\ \mathcal{E};\mathcal{P}\ \OD\ \FI\ \\
% 
&\Rightarrow & x:=x + y; \IF\ (x < 0)\ \THEN\ \ABORT; \ELSE\ \WHILE\ (x\neq y)
\ \DO\ (\mathcal{E}\ \mathcal{B}\ \mathcal{E});\mathcal{P}\ \OD\ \FI\ \\
% 
&\Rightarrow & x:=x + y; \IF\ (x < 0)\ \THEN\ \ABORT; \ELSE\ \WHILE\ (x\neq y)
\ \DO\ (\mathcal{V}+\mathcal{N});\mathcal{P}\ \OD\ \FI\ \\
% 
&\Rightarrow & x:=x + y; \IF\ (x < 0)\ \THEN\ \ABORT; \ELSE\ \WHILE\ (x\neq y)
\ \DO\ x := x + 1;\mathcal{P};\ \OD\ \FI\ \\
% 
&\Rightarrow & x:=x + y; \IF\ (x < 0)\ \THEN\ \ABORT; \ELSE\ \WHILE\ (x\neq y)
\ \DO\ x := x + 1;\mathcal{E};\ \OD\ \FI\ \\
% 
&\Rightarrow & x:=x + y; \IF\ (x < 0)\ \THEN\ \ABORT; \ELSE\ \WHILE\ (x\neq y)
\ \DO\ x := x + 1;(\mathcal{E}\ \mathcal{B}\ \mathcal{E});\ \OD\ \FI\ \\
% 
&\Rightarrow & x:=x + y; \IF\ (x < 0)\ \THEN\ \ABORT; \ELSE\ \WHILE\ (x\neq y)\ \DO
\ x := x + 1;(\mathcal{V} +\mathcal{N});\ \OD\ \FI\ \\
% 
&\Rightarrow & x:=x + y; \IF\ (x < 0)\ \THEN\ \ABORT; \ELSE\ \WHILE\ (x\neq y)\ \DO
\ x := x + 1;y := y + 2;\ \OD\ \FI\ \\
&&
\end{eqnarray*}

\end{small}
