$wp(x:=;$ if $x < 0$ then abort else while $x \neq y$ do $x:= x+1; y:=y+2;$
  od fi, $x=y) =$

$wp(x:=x+y,$ wp(if $x<0$ then abort else while $x \neq y$ do 
  $x:=x+1; y:=y+2;$ od fi, $x=y) =$

$wp($ if $x<0$ then abort else while $x \neq y$ do \dots od fi, $x=y) =$ \\
$=(( x<0 \Rightarrow \underbrace{wp(abort, x = y)}_{false} ) \land (x \geq 0 \Rightarrow wp($
  while $x \neq y$ do \dots od, $x=y)))$\\
$=(x<0 \Rightarrow false) \land (x \geq0 \Rightarrow wp(while  x\neq y$ 
  do \dots $od, x=y)) = $\\
$=(\underbrace{x<0 \land false}_{false}) \lor (x\geq 0 \land 
  wp(while x \neq y$ do \dots od $, x=y)) =$

$wp(while x\neq y$ do $x:=x+1; y:=y+2$ od $, x=y) =$\\


$\equiv $

$F_0 = (x=y \land x=y) = x=y$

$F_1 = (x\neq y \land wp(x:=x+1; y:=y+2, x=y)) = $
$ = x\neq y \land wp(x:=x+1, wp(y:=y+2, x=y)) = $\\
$ = x\neq y \land wp(x:=x+1, wp(y:=y+2, \underbrace{x=y}_{G})) = $\\
$ = x\neq y \land \underbrace{wp(x:=x+1, G[y|y+2])}_{**} = $
\begin{flushright} %right alligned
    ** \dots $G[y|y+2][x|x+1] \rightarrow (x+1 = y+2) \rightarrow x = y+1$
\end{flushright}
\noindent $ = x\neq y \land x=y+1 \Rightarrow x=y+1$

$F_2 = (x\neq y \land wp(x=x+1; y=y+1; \underbrace{x=y+1}_{G}))$\\
$ = (x\neq y \land G[y|y+2][x|x+1])$\\
$ = (x\neq y \land x+1 = y+2+1) = x=y+2$\\

\textbf{Guess:}\\

$F_i = (x\neq y \land x=y+i) = x=y+i$

$F_{i+1} = (x\neq y \land wp(x=x+1; y=y+2, x=y+1))$\\
$(x\neq y \land x=y+(i+1) = x=y+i+1)$\\


$wp(while x\neq y do$ \dots $od, x=y) =$\\
$= \exists i(i\geq 0\land x=y+i)$\\
$= i\geq 0 \land x-y=i$\\
$= x-y\geq 0$\\

$\Rightarrow wp(if x<0 then $ \dots $ fi, x=y)) =$\\
$ = (\underbrace{x<0 \land false}_{false} \lor 
  (x \geq 0 \land wp(while x\geq y do$ \dots $od, x=y))$\\
$false \lor (x\geq 0 \land x-y \geq 0)$\\
$(x\geq 0 \land x-y \geq 0)$\\

$\Rightarrow wp(x:=x+y, wp(if x<0 then)$ \dots $fi, x=y)) = $\\
$= wp(x:=x+y, x\geq 0 \land x-y\geq0)$\\
$= x\geq 0 \land (x+y)-y\geq 0$\\
$= x+y \geq 0 \land x\geq 0$


