%\solution{

\textbf{Description}\\
The function computes $\lfloor \sqrt[3]{a} \rfloor$

\vspace{0.5cm}

\begin{ALG}
\ASSERTN1{\text{Precondition: } a \ge 0}\\
\ASSERTN5{\INV \sub{c<-0} \sub{b<-1}}	\quad(as)$\ua$\\
$b \leftarrow 1;$\\
\ASSERTN4{\INV \sub{c<-0}}	\quad(as)$\ua$\\
$c \leftarrow 0;$\\
\ASSERTN3{\INV := b=(c+1)^3 \land 0 \le c^3 \le a}	\quad(wht'')\\
\WHILE\ $b \le a$ \DO\\
\ASSERTN8{\INV \land b \le a \land t=t_0}	\quad(wht'')\\
\ASSERTN{11}{\INV \land 0 \le t < t_0 \sub{b<-b+cd+1} \sub{c<-c+1} 
\sub{d<-3c+6}}	\quad(as)$\ua$\\
\>\ $d \leftarrow 3c+6;$\\
\ASSERTN{10}{\INV \land 0 \le t < t_0 \sub{b<-b+cd+1} \sub{c<-c+1}}	
\quad(as)$\ua$\\
\>\ $c \leftarrow c+1;$\\
\ASSERTN9{\INV \land 0 \le t < t_0 \sub{b<-b+cd+1}} \quad(as)$\ua$\\
\>\ $b \leftarrow b+cd+1;$\\
\ASSERTN7{\INV \land 0 \le t < t_0}	\quad(wht'')\\
\OD\\
\ASSERTN6{\INV \land b > a}	\quad(wht'')\\
\ASSERTN2{\text{Postcondition: } c^3 \le a < (c+1)^3}
\end{ALG}

\bigskip
\noindent We define the bound function $t$ as:\\
$t:=a-c$,\\
which fulfils the following criteria:\\
\begin{itemize}
\item
t must be an integer,
\item
t must be strictly monotonically nonincreasing,
\item
t must be greater or equal than 0.
\end{itemize}

\bigskip
\noindent To prove total correctness we have to show the following implications:\\´
\\
\textbf{$1 \rightarrow 5:$}\\
\indent $a \ge 0 \rightarrow Inv [c|0] [b|1]$\\
$= a \ge 0 \rightarrow b = (c+1)^3 \land 0 \le c^3 \le a [a|0] [b|1]$\\
$= a \ge 0 \rightarrow 1 = \underbrace{(0+1)^3}_{=1} \land 0 \le \underbrace{0^3}_{=0} \le a$\\
$=$ \sout{$a \ge 0$} $\rightarrow \underbrace{1 = 1}_{true} \checkmark\\
\indent \land$ \sout{$0 \le a$} \checkmark\\
\\
\textbf{$8 \rightarrow 11:$}\\
\indent $Inv \land b \le a \land t = t_0 \rightarrow Inv \land 0 \le t < t_0 [b|b+cd+1] [c|c+1] [d|3c+6]$\\
$= b = (c+1)^3 \land 0 \le c^3 \le a \land b \le a \land t = t_0\\ 
\indent \rightarrow b = (c+1)^3 \land 0 \le c^3 \le a \land 0 \le t < t_0 [b|b+cd+1] [c|c+1] [d|3c+6]$\\
$= b = (c+1)^3 \land 0 \le c^3 \le a \land b \le a \land t = t_0\\ 
\indent \rightarrow b + cd + 1 = (c+1)^3 \land 0 \le c^3 \le a \land 0 \le t < t_0 [c|c+1] [d|3c+6]$\\
$= b = (c+1)^3 \land 0 \le c^3 \le a \land b \le a \land t = t_0\\ 
\indent \rightarrow b + (c+1)d + 1 = (c+1+1)^3 \land 0 \le (c+1)^3 \le a \land 0 \le t < t_0 [d|3c+6]$\\
$= b = (c+1)^3 \land 0 \le c^3 \le a \land b \le a \land t = t_0\\ 
\indent \rightarrow b + (c+1)(3c+6) + 1 = (c+1+1)^3 \land 0 \le (c+1)^3 \le a \land 0 \le t < t_0$\\
$=$ \textcolor{green}{$b = (c+1)^3$} $\land 0 \le c^3 
\le a \land b \le a \land t = t_0\\ 
\indent \rightarrow b + (c+1)(3c+6) + 1 = (c+1+1)^3 
\land 0 \le$ \textcolor{green}{$\underbrace{(c+1)^3}_{=b}$} $\le a \land 0 \le \underbrace{t}_{=a-(c+1)} < \underbrace{t_0}_{=a-c}$\\
$= b = \underbrace{(c+1)^3}_{=c^3+3c^2+3c+1} \land$ \textcolor{magenta}{$0$} $\le c^3$ 
\textcolor{magenta}{$\le a$} $\land$ \textcolor{magenta}{$b \le a$} $\land t = t_0\\ 
\indent \rightarrow \underbrace{b + (c+1)(3c+6) + 1}_{=b+3c^2+9c+6+1} = \underbrace{(c+1+1)^3}_{=c^3+6c^2+12c+8} 
\land$ \textcolor{magenta}{$ 0 \le b \le a$} \\
\indent $\land 0 \le a-c-1 < a-c$ \checkmark \\
$= \textcolor{blue}{b = c^3+3c^2+3c+1} \land 0 \le c^3 \le a \land b \le a \land t = t_0\\ 
\indent \rightarrow \textcolor{blue}{b = c^3+3c^2+3c+1} \checkmark\\ 
\indent \land 0 \le b \le a \checkmark \\
\indent \land 0 \le a-c-1 < a-c$ \checkmark \\
\\
\textbf{$6 \rightarrow 2:$}\\
\indent $Inv \land b > a \rightarrow c^3 \le a < (c+1)^3$\\
$= b = (c+1)^3 \land 0 \le c^3 \le a \land b > a \rightarrow c^3 \le a < (c+1)^3$\\
$=$ \textcolor{green}{$b = (c+1)^3$} $\land 0 \le$ \sout{$c^3 \le a$} $\land b > a 
\rightarrow$ \sout{$c^3 \le a$} $<$ \textcolor{green}{$\underbrace{(c+1)^3}_{=b}$}\\
$= b = (c+1)^3 \land 0 \le c^3 \le a \land$ \textcolor{magenta}{$b > a$} 
$\rightarrow c^3 \le$ \textcolor{magenta}{$a < b$} \checkmark \\
\\
So the correctness asertion above is totally correct.
%}